Fixing build for main.v

concurrency/compiler/concurrent_compiler_simulation_proof.v
@@ -1,59 +1,136 @@
 Require Import compcert.common.Globalenvs.
+Require Import compcert.common.ExposedSimulations.
+Require Import compcert.common.Values.
+Require Import compcert.common.Memory.
 
+Require Import VST.concurrency.common.permissions.
 Require Import VST.concurrency.compiler.concurrent_compiler_simulation.
 Require Import VST.concurrency.compiler.sequential_compiler_correct.
 Require Import VST.concurrency.compiler.CoreSemantics_sum.
+Require Import VST.concurrency.common.HybridMachine.
+Require Import VST.concurrency.compiler.HybridMachine_simulation.
 
 
 (*Clight Machine *)
 Require Import VST.concurrency.common.ClightMachine.
 (*Asm Machine*)
 Require Import VST.concurrency.common.x86_context.
-
+(*
 
 (** *One thread simulation*)
-Module OneThreadSimulation (CC_correct: CompCert_correctness).
+Module ThreadedSimulation (CC_correct: CompCert_correctness).
   
   Import HybridMachineSig.
-
-  Module DMS.
-  Section DMS.
+  Import DryHybridMachine.
 
   Existing Instance OrdinalPool.OrdinalThreadPool.
-  Context (Clight_g : Clight.genv).
-  Definition CSem : Semantics := ClightSemantincsForMachines.ClightSem Clight_g.
-  
-  Import X86Context.
 
+  (** *C Semantics*)
+  Context (C_program: Clight.program).
+  Definition Clight_g : Clight.genv := Clight.globalenv C_program.
+  Definition CSem : Semantics := ClightSemantincsForMachines.ClightSem Clight_g.
+
+  
+  (** *Asm Semantics*)
+  Import X86Context.
   (*Import the Asm Hybrid Machine*)
-  Context (Asm_g : Clight.genv).
   Context (Asm_program: Asm.program).
+  Definition Asm_g := (@the_ge Asm_program).
   Context (Asm_genv_safe: Asm_core.safe_genv (@the_ge Asm_program)).
 
   
+  (** *AsHybrid Semantics and Machine*)
   Definition AsmSem : Semantics := @X86Sem Asm_program Asm_genv_safe.
 
   (** The hybrid semantics*)
-  Definition HybridSem h : Semantics := CoreSem_Sum h CSem AsmSem.
-
-  Existing Instance HybridMachine.DryHybridMachine.dryResources.
+  Instance HybridSem h : Semantics := CoreSem_Sum h CSem AsmSem.
+  Existing Instance dryResources.
   Notation TP h := (threadPool.OrdinalPool.OrdinalThreadPool(Sem:=HybridSem h)).
-  Existing Instance HybridMachine.DryHybridMachine.DryHybridMachineSig.
-
+  Existing Instance DryHybridMachineSig.
   Definition HybMachine h:=
     HybridMachineSig.HybridCoarseMachine.HybridCoarseMachine
       (ThreadPool:= TP h).
-
   Definition HybConcSem h:=
     HybridMachineSig.ConcurMachineSemantics(HybridMachine:=HybMachine h).
+  Notation ThreadPool n :=
+    (ThreadPool.t(Sem:= HybridSem n)).
 
+
+  (** *Extracting index and match relation from CompCert*)
+  Context (compiled: 
+             CC_correct.CompCert_compiler C_program = Some Asm_program).
+  Definition compiler_sim:= CC_correct.simpl_clight_semantic_preservation _ _ compiled.
+  Definition compiler_index: Type:= Injindex compiler_sim.
+  Definition compiler_match:= Injmatch_states compiler_sim.
+  
   Section CompileOneThread.
+    Import OrdinalPool.
+    Variable match_thread_source: forall n,
+        meminj -> @ctl (@semC (HybridSem (Some n))) -> mem -> @ctl (@semC (HybridSem (Some (S n)))) -> mem -> Prop.
+    Variable match_thread_target: forall n,
+        meminj -> @ctl (@semC (HybridSem (Some n))) -> mem -> @ctl (@semC (HybridSem (Some (S n)))) -> mem -> Prop.
+    Inductive match_thread_compiled n:
+      option compiler_index -> meminj -> @ctl (@semC (HybridSem (Some n))) -> mem -> @ctl (@semC (HybridSem (Some (S n)))) -> mem -> Prop  :=
+    | Build_match_thread_compiled:
+        forall i j st1 m1 st2 m2,
+        compiler_match i j (Smallstep.set_mem st1 m1) (Smallstep.set_mem st2 m2) ->
+        match_thread_compiled n (Some i) j st1 m1 st2 m2.
+      
+
+  Definition FST {A B} (HH : A /\ B):=
+    fst (ssrfun.pair_of_and HH).
+
+  Definition SND {A B} (HH : A /\ B):=
+    snd (ssrfun.pair_of_and HH).
+    
+    Record concur_match hb (ocd: option compiler_index)
+       (j:meminj) (cstate1: ThreadPool (Some hb)) (m1: Mem.mem) (cstate2: ThreadPool(Some (S hb))) (m2: mem):=
+  { same_length: num_threads cstate1 = num_threads cstate2
+    ; memcompat1: mem_compatible cstate1 m1
+    ; memcompat2: mem_compatible cstate2 m2
+    ; mtch_source:
+        forall (i:nat),
+          (i > hb)%nat ->
+          forall (cnti1: containsThread cstate1 i)
+            (cnti2: containsThread cstate2 i),
+          match_thread_source hb j
+                              (getThreadC cnti1)
+                              (permissions.restrPermMap (FST (memcompat1 i cnti1)))
+                              (getThreadC cnti2)
+                              (permissions.restrPermMap (FST (memcompat2 i cnti2)))
+    ; mtch_target:
+        forall (i:nat),
+          (i < hb)%nat ->
+          forall (cnti1: containsThread cstate1 i)
+            (cnti2: containsThread cstate2 i),
+          match_thread_target  hb j
+                              (getThreadC cnti1)
+                              (restrPermMap (FST(memcompat1 i cnti1)))
+                              (getThreadC cnti2)
+                              (permissions.restrPermMap (FST(memcompat2 i cnti2)))
+    ; mtch_compiled:
+        forall (i:nat),
+          (i = hb)%nat ->
+          forall (cnti1: containsThread cstate1 i)
+            (cnti2: containsThread cstate2 i),
+            exists cd, ocd = Some cd /\
+                  match_thread_compiled cd j
+                                (getThreadC cnti1)
+                                (restrPermMap (FST(memcompat1 i cnti1)))
+                                (getThreadC cnti2)
+                                (restrPermMap (FST(memcompat2 i cnti2))) }.
+    
+    Variable match_state: forall n,
+      index ->
+      Values.Val.meminj ->
+      ThreadPool (Some n) -> Memory.Mem.mem -> ThreadPool (Some (S n)) -> Memory.Mem.mem -> Prop.
     
     Lemma compile_one_thread:
       forall n m,
-        HybridMachine_simulation.HybridMachine_simulation
+        HybridMachine_simulation_properties
           (HybConcSem (Some n) m)
-          (HybConcSem (Some (S n)) m).
+          (HybConcSem (Some (S n)) m)
+          (match_state n).
     Proof.
       intros.
     Admitted.
@@ -61,23 +138,54 @@ Module OneThreadSimulation (CC_correct: CompCert_correctness).
   End CompileOneThread.
 
   
-  Section CompileNThread.
-  
+  Section CompileNThreads.
+
+    
+ Variable index: nat -> Type.
+ Variable match_state: forall n,
+     index n ->
+     Values.Val.meminj ->
+     ThreadPool (Some 0) -> Memory.Mem.mem -> ThreadPool (Some n) -> Memory.Mem.mem -> Prop.
+ 
   Lemma compile_n_threads:
       forall n m,
-        HybridMachine_simulation.HybridMachine_simulation
+        HybridMachine_simulation.HybridMachine_simulation_properties
           (HybConcSem (Some 0) m)
-          (HybConcSem (Some n) m).
+          (HybConcSem (Some n) m)
+          (match_state n).
     Proof.
       intros.
     Admitted.
 
-  End CompileNThread.
+  End CompileNThreads.
 
+ Section CompileInftyThread.
+    
+ Variable index: nat -> Type.
+ Variable match_state: forall n,
+     index n ->
+     Values.Val.meminj ->
+     ThreadPool (Some 0) -> Memory.Mem.mem -> ThreadPool (Some n) -> Memory.Mem.mem -> Prop.
+ 
+  Lemma compile_all_threads:
+      forall n m,
+        HybridMachine_simulation.HybridMachine_simulation_properties
+          (HybConcSem (Some 0) m)
+          (HybConcSem None m)
+          (match_state n).
+    Proof.
+      intros.
+    Admitted.
+
+  End CompileInftyThread.
+
+
+
+  
   
       
   
-  Lemma ConcurrentCompilerCorrectness:
+(*  Lemma ConcurrentCompilerCorrectness:
     forall (p:Clight.program) (tp:Asm.program),
       CC_correct.CompCert_compiler p = Some tp ->
       forall asm_genv_safety,
@@ -92,8 +200,8 @@ Module OneThreadSimulation (CC_correct: CompCert_correctness).
     unfold ClightMachine.ClightMachine.DMS.ClightConcurSem, HybridMachineSig.HybridMachineSig.ConcurMachineSemantics, ClightMachine.ClightMachine.DMS.ClightMachine, HybridMachineSig.HybridMachineSig.HybridCoarseMachine.HybridCoarseMachine.
     econstructor.
 *)
-
-
+End ThreadedSimulation.
+  *)
 Module Concurrent_correctness (CC_correct: CompCert_correctness).
 
   
